CD without constants

theories/FOcdint/FO_CDInt_Conservativity.v
@@ -4,23 +4,33 @@ Require Import PeanoNat.
 Require Import Lia.
 Require Import Ensembles.
 Require Import Arith.
+Require Import Coq.Vectors.Vector.
+Local Notation vec := Vector.t.
 
 Require Import FO_BiInt_Syntax.
 Require Import FO_BiInt_GHC.
+Require Import FO_BiInt_Kripke_sem.
 Require Import FO_BiInt_soundness.
 
 Require Import FO_CDInt_Syntax.
 Require Import FO_CDInt_GHC.
 Require Import FO_CDInt_logic.
 Require Import FOCDIH_properties.
-Require Import FO_CDInt_Lindenbaum_lem.
+Require Import FO_CDInt_Stand_Lindenbaum_lem.
+Require Import FO_CDInt_Up_Lindenbaum_lem.
 Require Import FO_CDInt_Kripke_sem.
 Require Import FO_CDInt_completeness.
 
 Section conservativity.
 
-Context {Σ_funcs : funcs_signature}.
-Context {Σ_preds : preds_signature}.
+Context {Σ_funcs : FO_CDInt_Syntax.funcs_signature}.
+Context {Σ_preds : FO_CDInt_Syntax.preds_signature}.
+
+
+Instance biΣ_funcs : FO_BiInt_Syntax.funcs_signature :=
+  {| FO_BiInt_Syntax.syms := Σ_funcs; FO_BiInt_Syntax.ar_syms := (@ar_syms Σ_funcs) |}.
+Instance biΣ_preds : FO_BiInt_Syntax.preds_signature :=
+  {| FO_BiInt_Syntax.preds := Σ_preds; FO_BiInt_Syntax.ar_preds := (@ar_preds Σ_preds) |}.
 
 Variable eq_dec_preds : forall x y : preds, {x = y}+{x <> y}.
 Variable eq_dec_funcs : forall x y : Σ_funcs, {x = y}+{x <> y}.
@@ -28,25 +38,24 @@ Variable eq_dec_funcs : forall x y : Σ_funcs, {x = y}+{x <> y}.
 Fixpoint embed_term (t : term) : FO_BiInt_Syntax.term :=
   match t with 
   | var n => FO_BiInt_Syntax.var n
-  | cst n => FO_BiInt_Syntax.var 42 (* dummy *)
-  | func f v => FO_BiInt_Syntax.func f (Vector.map embed_term v)
+  | func f v => FO_BiInt_Syntax.func biΣ_funcs f (Vector.map embed_term v)
   end.
 
-Definition embed_bin (b : full_logic_sym) : @binop FO_BiInt_Syntax.FullSyntax.full_operators :=
+Definition embed_bin (b : full_logic_sym) : @FO_BiInt_Syntax.binop FO_BiInt_Syntax.FullSyntax.full_operators :=
   match b with 
   | Conj => FO_BiInt_Syntax.FullSyntax.Conj
   | Disj => FO_BiInt_Syntax.FullSyntax.Disj
   | Impl => FO_BiInt_Syntax.FullSyntax.Impl
   end.
 
-Definition embed_quant (q : full_logic_quant) : @quantop FO_BiInt_Syntax.FullSyntax.full_operators :=
+Definition embed_quant (q : full_logic_quant) : @FO_BiInt_Syntax.quantop FO_BiInt_Syntax.FullSyntax.full_operators :=
   match q with 
   | All => FO_BiInt_Syntax.FullSyntax.All
   | Ex => FO_BiInt_Syntax.FullSyntax.Ex
   end.
 
 Definition form' :=
-  @FO_BiInt_Syntax.form Σ_funcs Σ_preds FO_BiInt_Syntax.FullSyntax.full_operators.
+  @FO_BiInt_Syntax.form biΣ_funcs biΣ_preds FO_BiInt_Syntax.FullSyntax.full_operators.
 
 Fixpoint embed (phi : form) : form' :=
   match phi with
@@ -60,37 +69,60 @@ Fixpoint embed (phi : form) : form' :=
 
 Variable form_enum : nat -> form.
 Variable form_enum_sur : forall A, exists n, form_enum n = A.
-Variable form_enum_cunused : forall n, forall A m, form_enum m = A -> m <= n -> cunused n A.
 Variable form_index : form -> nat.
 Variable form_enum_index : forall A, form_enum (form_index A) = A.
+Variable form_enum_unused : forall n, forall A m, form_enum m = A -> m <= n -> unused n A.
 Variable form_index_inj : forall A B, form_index A = form_index B -> A = B.
 
-Lemma embed_eval D (I : interp D) (a : ass D) rho (t : term) :
-  cst_free_term t -> eval rho t = FO_BiInt_Kripke_sem.eval rho (embed_term t).
+Instance biinterp D (I : interp D) : FO_BiInt_Kripke_sem.interp D :=
+      {|
+        FO_BiInt_Kripke_sem.i_func := fun (f : biΣ_funcs) (v: vec D ((@FO_BiInt_Syntax.ar_syms biΣ_funcs) f)) => (@i_func _ _ I) f v
+      |}.
+
+Lemma embed_eval D (I : interp D) rho (t : term) :
+   @FO_CDInt_Kripke_sem.eval _ D I rho t = @FO_BiInt_Kripke_sem.eval _ D (biinterp _ I) rho (embed_term t).
 Proof.
-  induction t using strong_term_ind; inversion 1; subst; cbn; try reflexivity.
-  rewrite Vector.map_map. erewrite vec_map_ext; try reflexivity. intros t' Ht.
-  apply H; trivial. apply H2. unshelve eapply inj_right_pair in H3; subst; trivial.
+  induction t using strong_term_ind.
+  - cbn ; auto.
+  - cbn. rewrite Vector.map_map. erewrite vec_map_ext; try reflexivity. intros t' Ht.
+    apply H; trivial.
 Qed.
 
-Lemma embed_ksat D (M : kmodel D) (a : ass D) w rho (phi : form) :
-  cst_free phi -> (M ⊩( a, D) w) rho phi <-> FO_BiInt_Kripke_sem.ksat w rho (embed phi).
+Instance bikmodel D (M : kmodel D) : FO_BiInt_Kripke_sem.kmodel D :=
+      {|
+        FO_BiInt_Kripke_sem.nodes := (@nodes _ _ _ M) ;
+
+        FO_BiInt_Kripke_sem.reachable := (@reachable _ _ _ M) ;
+        FO_BiInt_Kripke_sem.reach_refl u := (@reach_refl _ _ _ M) u ;
+        FO_BiInt_Kripke_sem.reach_tran u v w := (@reach_tran _ _ _ M) u v w ;
+
+        FO_BiInt_Kripke_sem.k_interp := biinterp D (@k_interp _ _ _ M)  ;
+        FO_BiInt_Kripke_sem.k_P n P v := (@k_P _ _ _ M) n P v ;
+
+        FO_BiInt_Kripke_sem.mon_P u v uRv P t ut := (@mon_P _ _ _ M) u v uRv P t ut ;
+      |}.
+
+Lemma embed_ksat D (M : kmodel D) w rho (phi : form) :
+    (w ⊩(M,D) rho) phi <-> FO_BiInt_Kripke_sem.ksat w rho (embed phi).
 Proof.
-  induction phi in w, rho |- *; inversion 1; subst; try destruct b; try destruct q; cbn.
-  all: try now intuition.
-  - rewrite Vector.map_map. erewrite vec_map_ext; try reflexivity. intros t' Ht.
-    apply embed_eval. apply H1. unshelve eapply inj_right_pair in H2; subst; trivial.
-  - firstorder.
+  induction phi in w, rho |- *.
+  - cbn ; intuition.
+  - cbn. rewrite Vector.map_map. erewrite vec_map_ext; try reflexivity. intros t' Ht.
+    apply embed_eval.
+  - destruct b ; cbn. 1-2: firstorder.
+    split ; intros ; apply IHphi2 ; apply H ; auto ; apply IHphi1 ; auto.
+  - destruct q ; cbn ; firstorder.
 Qed.
 
 Variable SLEM : forall P : Prop, P + ~ P.
-Variable w_all : forall (w : cworlds) (A : form), ~ w (∀ A) -> {c : nat | ~ w A[#c..]}.
 
-Theorem conservativity (phi : form) :
-  cst_free phi -> FOBIH_prv (Empty_set _) (embed phi) -> FOCDIH_prv (Empty_set _) phi.
+Theorem conservativity : forall X A, closed_S X -> closed A ->
+   FOBIH_prv (fun x => exists y, X y /\ x = embed y) (embed A) -> FOCDIH_prv X A.
 Proof.
-  intros H1 H2. eapply completeness; eauto.
-  intros D a M w rho _. apply embed_ksat; trivial. apply Soundness in H2. apply H2. intros B [].
+  intros X A CX CA H. eapply Completeness; eauto.
+  intros D M w rho H1. apply embed_ksat; trivial. apply Soundness in H. apply H.
+  intros B HB. destruct HB as (C & H2 & H3) ; subst.
+  apply embed_ksat ; auto.
 Qed.
 
 End conservativity.
