theories/FOcdint/FO_CDInt_completeness.v
@@ -1,9 +1,3 @@
-Require Import Classical.
-(* Used in various places:
-    - existence of a derivation in the axiomatic system for a sequent
-      (should be decidable as Bi-Int is, but this would require extra work)
-    - some set-theoretic arguments (maybe they can be constructivised *)
-
 Require Import FunctionalExtensionality.
 
 Require Import List.
@@ -17,10 +11,18 @@ Require Import FO_CDInt_Syntax.
 Require Import FO_CDInt_GHC.
 Require Import FO_CDInt_logic.
 Require Import FOCDIH_properties.
-Require Import FO_CDInt_Lindenbaum_lem.
+Require Import FO_CDInt_Stand_Lindenbaum_lem.
+Require Import FO_CDInt_Up_Lindenbaum_lem.
 Require Import FO_CDInt_Kripke_sem.
 
 Section completeness.
+
+Variable SLEM : forall P : Prop, P + ~ P.
+
+Corollary LEM : forall P : Prop, P \/ ~ P.
+Proof.
+intro P ; destruct (SLEM P) ; auto.
+Qed.
 
   Context {Σ_funcs : funcs_signature}.
   Context {Σ_preds : preds_signature}.
@@ -32,12 +34,14 @@ Variable eq_dec_funcs : forall x y : Σ_funcs, {x = y}+{x <> y}.
 
 Variable form_enum : nat -> form.
 Variable form_enum_sur : forall A, exists n, form_enum n = A.
-Variable form_enum_cunused : forall n, forall A m, form_enum m = A -> m <= n -> cunused n A.
+Variable form_enum_unused : forall n, forall A m, form_enum m = A -> m <= n -> unused n A.
 Variable form_index : form -> nat.
 Variable form_enum_index : forall A, form_enum (form_index A) = A.
 Variable form_index_inj : forall A B, form_index A = form_index B -> A = B.
 
-
+Notation "x 'el' L" := (List.In x L) (at level 70).
+Notation "T |- phi" := (FOCDIH_prv T phi) (at level 80).
+Notation adj T phi := (fun psi => T psi \/ psi = phi).
 
 (* Canonical model construction *)
 
@@ -54,12 +58,9 @@ Coercion cX : cworlds >-> Funclass.
 Instance universal_interp : interp term :=
     {| i_func := func  |}.
 
-Instance cst_ass : ass term := cst.
-
 Lemma universal_interp_eval rho (t : term) : eval rho t = t `[rho].
 Proof.
-induction t using term_ind ; auto. simpl. f_equal.
-apply Vector.map_ext_in. intros. apply IH. auto.
+induction t using term_ind ; auto.
 Qed.
 
 Lemma universal_interp_eval0 n (t : Vector.t term n): (Vector.map (eval var) t) = t.
@@ -77,551 +78,49 @@ Program Instance Canon_model : kmodel term :=
         k_P := fun C P v => C (atom P v)
       |}.
 
-Lemma Lind1 : forall A, cst_free A -> ~ FOCDIH_prv (Empty_set _) A ->
-      exists (cw : cworlds), ~ cw A.
+Lemma cwTradLind : forall X A, closed_S X -> closed A -> ~ (FOCDIH_prv X A) ->
+      exists (cw : cworlds), ~ cw A /\ Included _ X cw.
 Proof.
 intros.
-eapply Lindenbaum_lemma in H0 ; auto.
-destruct H0 as (X & notin & ded & prim & exh & allh & notder).
-epose (Build_cworlds X _ prim ded exh allh). exists c.
-intro. apply notin. auto.
-apply form_enum_cunused.
+assert (~ pair_der X (Singleton _ A)).
+{ intro. destruct H2 as (l & Hl0 & Hl1 & Hl2).
+  apply H1. apply forall_list_disj with l ; auto.
+  intros. apply Hl1 in H2. inversion H2 ; subst. apply
+  imp_Id_gen. }
+eapply Stand_Lindenbaum_lemma_pair in H2 ; auto.
+destruct H2. repeat destruct p.
+epose (Build_cworlds x _ p0 d e a). exists c. split.
+intro. apply n. exists [A]. repeat split.
+apply NoDup_cons ; auto. apply NoDup_nil.
+intros B HB. inversion HB ; subst. split.
+inversion H3. cbn. eapply MP.
+apply Ax ; eapply A3 ; reflexivity. apply Id ; auto.
+intros B HB. apply i ; auto.
+apply LEM.
+apply form_enum_unused.
+intros B HB. inversion HB ; subst ; auto.
 Unshelve.
-intro D. apply notder.
-eapply MP. apply EFQ. auto.
+intro D. apply n.
+exists [] ; cbn ; repeat split ; auto.
+apply NoDup_nil. intros ; contradiction.
 Qed.
 
-Variable SLEM : forall P : Prop, P + ~ P.
-
-Notation "x 'el' L" := (List.In x L) (at level 70).
-Notation "T |- phi" := (FOCDIH_prv T phi) (at level 80).
-Notation adj T phi := (fun psi => T psi \/ psi = phi).
-
-Section Prv.
-
-  Lemma prv_ctx (T : form -> Prop) phi :
-    T phi -> T |- phi.
-  Proof.
-    intros H. apply Id. auto.
-  Qed.
-
-  Lemma prv_weak T T' A :
-    T |- A -> Included _ T T' -> T' |- A.
-  Proof.
-    intros H1 H2. eapply FOCDIH_monot in H1; eassumption.
-  Qed.
-
-  Lemma prv_MP {T : form -> Prop} {phi} psi :
-    T |- psi --> phi -> T |- psi -> T |- phi.
-  Proof.
-    intros H1 H2. eapply MP ; auto.
-    - exact H1.
-    - auto.
-  Qed.
-
-  Lemma prv_DT T A B :
-    adj T A |- B <-> T |- A --> B.
-  Proof.
-    split; intros HT.
-    - apply FOCDIH_Deduction_Theorem.
-      eapply prv_weak; try apply HT. intros C [HC| ->]; [ left | right ]; trivial. constructor.
-    - apply prv_MP with A; try (apply prv_ctx; now right). eapply prv_weak; try apply HT. firstorder.
-  Qed.
-
-  Lemma prv_compact T A :
-    T |- A -> exists L, (forall B, B el L -> T B) /\ (fun B => B el L) |- A.
-  Proof.
-    intros (T' & H1 & H2 & L & HL) % FOCDIH_finite. exists L. split; intuition.
-    eapply prv_weak; try apply H2. intuition.
-  Qed.
-
-  Lemma prv_cut T T' A :
-    T |- A -> (forall B, T B -> T' |- B) -> T' |- A.
-  Proof.
-    intros [L [H1 H2]] % prv_compact H. induction L in A, H1, H2 |- *.
-    - eapply prv_weak; try apply H2. intros B [].
-    - eapply prv_MP; try apply (IHL (a --> A)).
-      + intros B HB. apply H1. now right.
-      + apply prv_DT. eapply prv_weak; try apply H2. intros B [->| HB]; cbn; intuition.
-      + apply H, H1. now left.
-  Qed.
-
-  Lemma prv_EI {T : form -> Prop} {phi} t :
-    T |- phi[t..] -> T |- ∃ phi.
-  Proof.
-    intros H. eapply prv_MP; try apply H. constructor 2.
-    econstructor 12 ; reflexivity.
-  Qed.
-
-   Lemma prv_EE T A B :
-    (fun C => exists C', C = C'[↑] /\ T C') |- A --> B[↑] -> T |- (∃ A) --> B.
-  Proof.
-    intros H. eapply EC; try apply ECRule_I ; auto.
-  Qed.
-
-  Lemma prv_AI T A :
-    (fun C => exists C', C = C'[↑] /\ T C') |- A -> T |- ∀ A.
-  Proof.
-    intros H. eapply Gen; try apply GenRule_I ; auto.
-  Qed.
-
-  Lemma prv_AE {T : form -> Prop} {phi} t :
-    T |- ∀ phi -> T |- phi[t..].
-  Proof.
-    intros H. eapply prv_MP; try apply H. constructor 2.
-    econstructor 11 ; reflexivity.
-  Qed.
-
-  Lemma prv_DI1 T A B :
-    T |- A -> T |- A ∨ B.
-  Proof.
-    intros H. eapply prv_MP; try apply H. constructor 2.
-    econstructor 3 ; reflexivity.
-  Qed.
-
-  Lemma prv_DI2 T A B :
-    T |- B -> T |- A ∨ B.
-  Proof.
-    intros H. eapply prv_MP; try apply H. constructor 2.
-    econstructor 4 ; reflexivity.
-  Qed.
-
-  Lemma prv_DE T phi psi theta :
-    T |- phi ∨ psi -> adj T phi |- theta -> adj T psi |- theta -> T |- theta.
-  Proof.
-    intros H1 H2 H3. eapply prv_MP. eapply prv_MP. eapply prv_MP.
-    - constructor 2. econstructor 5 ; reflexivity.
-    - apply prv_DT. apply H2.
-    - apply prv_DT. apply H3.
-    - apply H1.
-  Qed.
-
-  Lemma prv_CI T A B :
-    T |- A -> T |- B -> T |- A ∧ B.
-  Proof.
-    intros H1 H2. eapply prv_MP. eapply prv_MP. eapply prv_MP.
-    - constructor 2. econstructor 8 ; reflexivity.
-    - apply prv_DT. apply prv_ctx. now right.
-    - eapply MP. apply Thm_irrel. auto.
-    - apply H1.
-  Qed.
-
-  Lemma prv_CE1 T A B :
-    T |- A ∧ B -> T |- A.
-  Proof.
-    intros H. eapply prv_MP; try apply H. constructor 2.
-    econstructor 6 ; reflexivity.
-  Qed.
-
-  Lemma prv_CE2 T A B :
-    T |- A ∧ B -> T |- B.
-  Proof.
-    intros H. eapply prv_MP; try apply H. constructor 2.
-    econstructor 7 ; reflexivity.
-  Qed.
-
-  Lemma prv_exp T A :
-    T |- ⊥ -> T |- A.
-  Proof.
-    intros H. eapply prv_MP; try apply H. constructor 2.
-    econstructor 9 ; reflexivity.
-  Qed.
-
-  Lemma prv_cas_car T A B C :
-    T |- A --> B --> C <-> T |- B ∧ A --> C.
-  Proof.
-    split; intros H.
-    - apply prv_DT. eapply prv_MP. eapply prv_MP.
-      + eapply prv_weak; try apply H. firstorder.
-      + eapply prv_CE2, prv_ctx. now right.
-      + eapply prv_CE1, prv_ctx. now right.
-    - apply prv_DT. apply -> prv_DT. eapply prv_MP.
-      + eapply prv_weak; try apply H. firstorder.
-      + apply prv_CI; apply prv_ctx; firstorder.
-  Qed.
-
-  Lemma prv_list_conj T L :
-    (forall A, A el L -> T |- A) -> T |- list_conj L.
-  Proof.
-    intros H. induction L.
-    - apply prv_Top.
-    - cbn. apply prv_CI.
-      + apply H. now left.
-      + apply IHL. firstorder.
-  Qed.
-
-  Lemma prv_list_conj' T L A :
-    A el L -> adj T (list_conj L) |- A.
-  Proof.
-    induction L; cbn; try tauto. intros [-> | H].
-    - eapply prv_CE1. apply prv_ctx. now right.
-    - apply prv_DT in IHL; trivial. eapply prv_MP.
-      + eapply prv_weak; try apply IHL. firstorder.
-      + eapply prv_CE2. apply prv_ctx. now right.
-  Qed.
-
-  Lemma prv_list_disj T L A :
-    A el L -> T |- A -> T |- list_disj L.
-  Proof.
-    induction L; cbn; try now intros []. intros [-> |H] HA.
-    - apply prv_DI1. apply HA.
-    - apply prv_DI2. now apply IHL.
-  Qed.
-
-  Lemma list_disj_mono T L L' :
-    incl L L' -> T |- list_disj L -> T |- list_disj L'.
-  Proof.
-    induction L in T |- *; cbn; intros H1 H2.
-    - apply prv_exp. apply H2.
-    - eapply prv_DE; try apply H2.
-      + apply prv_list_disj with a; try firstorder. apply prv_ctx. now right.
-      + apply IHL; try firstorder. apply prv_ctx. now right.
-  Qed.
-
-  Lemma Lext_ex_der {T L1 L2 psi} c :
-    T |- list_conj (∃ psi :: psi[#c..] :: L1) --> list_disj L2
-        -> T |- list_conj L1 --> psi[#c..] --> list_disj L2.
-  Proof.
-    intros H. apply prv_DT. apply -> prv_DT. apply prv_DT in H.
-    eapply prv_cut; try apply H. intros B [HB | ->].
-    - apply prv_ctx. left. now left.
-    - cbn. apply prv_CI; try apply prv_CI.
-      + eapply prv_EI. apply prv_ctx. now right.
-      + apply prv_ctx. now right.
-      + apply prv_ctx. left. now right.
-  Qed.
-
-  Lemma Lext_all_der {T L1 L2 psi} c :
-    T |- list_conj L1 --> list_disj (∀ psi :: psi[#c..] :: L2)
-        -> T |- list_conj L1 --> psi[#c..] ∨ list_disj L2.
-  Proof.
-    intros H. apply prv_DT. apply prv_DT in H.
-    cbn in H. eapply prv_DE; try apply H.
-    - apply prv_DI1. apply prv_AE. apply prv_ctx. now right.
-    - apply prv_ctx. now right.
-  Qed.
-
-End Prv.
-
-Section Lind2.
-
-  Variable w : cworlds.
-  Variable A0 B0 : form.
-
-  Variable w_all : forall A, ~ w (∀ A) -> { c : nat | ~ w A[#c..] }.
-  Hypothesis w_nder : ~ FOCDIH_prv (fun x => w x \/ x = A0) B0.
-
-  Lemma form_all phi :
-    { psi | phi = ∀ psi } + (~ exists psi, phi = ∀ psi).
-  Proof.
-    destruct phi; try destruct q. 1-3,5: right; intros [psi H]; discriminate.
-    left. exists phi. reflexivity.
-  Qed.
-
-  Lemma form_ex phi :
-    { psi | phi = ∃ psi } + (~ exists psi, phi = ∃ psi).
-  Proof.
-    destruct phi; try destruct q. 1-4: right; intros [psi H]; discriminate.
-    left. exists phi. reflexivity.
-  Qed.
-
-  Lemma form_subst_help phi :
-    phi[up ↑][$0..] = phi.
-  Proof.
-    rewrite subst_comp. apply subst_id. now intros [].
-  Qed.
-
-  Lemma Lext_all {L1 L2 psi} :
-    ~ FOCDIH_prv cX (list_conj L1 --> (∀ psi) ∨ list_disj L2)
-    -> { c | ~ cX (list_conj L1 --> psi[#c..] ∨ list_disj L2) }.
-  Proof.
-    intros HD. assert (~ cX (∀ (list_conj L1)[↑] --> psi ∨ (list_disj L2)[↑])).
-    - intros H. apply HD. apply prv_ctx in H. apply prv_DT. eapply prv_MP.
-      + constructor 2. econstructor 13 ; reflexivity.
-      + apply prv_AI. eapply FOCDIH_subst in H. Unshelve. 2: exact ↑. cbn in H.
-        apply prv_AE with $0 in H. cbn in H. rewrite !form_subst_help in H.
-        apply <- prv_DT in H. apply (FOCDIH_monot _ _ H). cbn.
-        intros A [[B [-> HA]]| ->].
-        * exists B. split; trivial. constructor. apply HA.
-        * exists (list_conj L1). split; trivial. constructor 2. reflexivity.
-    - apply w_all in H as [c Hc]. cbn in Hc. rewrite !subst_shift in Hc. exists c. apply Hc.
-  Defined.
-
-  Lemma Lext_ex {L1 L2 psi} :
-    ~ FOCDIH_prv cX (list_conj L1 --> (∃ psi) --> list_disj L2)
-    -> { c | ~ cX (list_conj L1 --> psi[#c..] --> list_disj L2) }.
-  Proof.
-    intros HD. assert (~ cX (∀ (list_conj L1)[↑] --> psi --> (list_disj L2)[↑])).
-    - intros H. apply HD. apply prv_ctx in H. apply prv_DT.
-      apply prv_EE. eapply FOCDIH_subst in H. Unshelve. 2: exact ↑. cbn in H.
-      apply prv_AE with $0 in H. cbn in H. rewrite !form_subst_help in H.
-      apply <- prv_DT in H. apply (FOCDIH_monot _ _ H). cbn.
-      intros A [[B [-> HA]]| ->].
-      + exists B. split; trivial. constructor. apply HA.
-      + exists (list_conj L1). split; trivial. constructor 2. reflexivity.
-    - apply w_all in H as [c Hc]. cbn in Hc. rewrite !subst_shift in Hc. exists c. apply Hc.
-  Qed.
-
-  Fixpoint Lext (n : nat) : list form * list form :=
-    match n with
-    | 0 => ([A0], [B0])
-    | S n => let (L1, L2) := Lext n in let phi := form_enum n in
-            match form_all phi, form_ex phi with 
-            | inl (exist _ psi _), _ => match SLEM (cX |- (list_conj L1) --> (∀ psi) ∨ list_disj L2) with
-                                     | inl _ => (∀ psi :: L1, L2)
-                                     | inr H => (L1, ∀ psi :: psi[#(proj1_sig (Lext_all H))..] :: L2)
-                                     end
-            | _, inl (exist _ psi _) => match SLEM (cX |- (list_conj L1) --> (∃ psi) --> list_disj L2) with
-                                     | inl _ => (L1, ∃ psi :: L2)
-                                     | inr H => (∃ psi :: psi[#(proj1_sig (Lext_ex H))..] :: L1, L2)
-                                     end
-            | _, _ => if SLEM (cX |- list_conj (phi :: L1) --> list_disj L2)
-                     then (L1, phi :: L2) else (phi :: L1, L2)
-            end
-    end.
-
-  Lemma Lext_cum1 n n' :
-    n <= n' -> incl (fst (Lext n)) (fst (Lext n')).
-  Proof.
-    induction 1. firstorder. intros phi HP. cbn. destruct (Lext m) eqn: HL.
-    destruct form_all as [[]|]; try destruct form_ex as [[]|]; destruct SLEM.
-    all: cbn ; auto.
-  Qed.
-
-  Lemma Lext_cum2 n n' :
-    n <= n' -> incl (snd (Lext n)) (snd (Lext n')).
-  Proof.
-    induction 1. firstorder. intros phi HP. cbn. destruct (Lext m) eqn: HL.
-    destruct form_all as [[]|]; try destruct form_ex as [[]|]; destruct SLEM.
-    all: cbn ; auto.
-  Qed.
-
-  Lemma Lext_nder n :
-    ~ (cX |- list_conj (fst (Lext n)) --> list_disj (snd (Lext n))).
-  Proof.
-    induction n; intros HD.
-    - cbn in HD. apply w_nder. eapply prv_DE.
-      + eapply prv_MP; try apply (prv_weak _ _ _ HD); try firstorder. apply prv_CI.
-        * apply prv_ctx. now right.
-        * apply prv_Top.
-      + apply prv_ctx. now right.
-      + apply prv_exp. apply prv_ctx. now right.
-    - cbn in *. destruct Lext, form_all as [[]|]; try destruct form_ex as [[]|];
-        destruct SLEM; try destruct Lext_all; try destruct Lext_ex; subst; cbn in *.
-      + apply IHn. apply prv_DT. apply prv_DT in f. eapply prv_DE; try apply f.
-        * apply prv_DT, prv_DT. apply prv_cas_car. apply HD.
-        * apply prv_ctx. now right.
-      + apply Lext_all_der, cded_clos in HD. contradiction.
-      + apply IHn. apply prv_DT. apply prv_DT in HD. eapply prv_DE; try apply HD.
-        * apply prv_DT, prv_DT. apply f.
-        * apply prv_ctx. now right.
-      + apply Lext_ex_der, cded_clos in HD. contradiction.
-      + apply IHn. apply prv_DT. apply prv_DT in HD. eapply prv_DE; try apply HD.
-        * apply prv_DT, prv_DT. apply prv_cas_car. apply f.
-        * apply prv_ctx. now right.
-      + apply n2. apply HD.
-  Qed.
-
-  Lemma Lext_A0 n :
-    A0 el fst (Lext n).
-  Proof.
-    induction n; cbn; try tauto.
-    destruct (Lext n) as [L1 L2]. cbn in IHn.
-    destruct form_all as [[]|]; try destruct form_ex as [[]|]; destruct SLEM; cbn; tauto.
-  Qed.
-
-  Lemma Lext_B0 n :
-    B0 el snd (Lext n).
-  Proof.
-    induction n; cbn; try tauto.
-    destruct (Lext n) as [L1 L2]. cbn in IHn.
-    destruct form_all as [[]|]; try destruct form_ex as [[]|]; destruct SLEM; cbn; tauto.
-  Qed.
-
-  Definition ext phi :=
-    w phi \/ exists n, phi el fst (Lext n).
-
-  Lemma ext_der n :
-    ext |- list_conj (fst (Lext n)).
-  Proof.
-    apply prv_list_conj. intros A HA. apply prv_ctx. right. now exists n.
-  Qed.
-
-  Lemma ext_prv phi :
-    ext |- phi -> exists n, (fun psi => cX psi \/ psi el fst (Lext n)) |- phi.
-  Proof.
-    intros [L[H1 H2]] % prv_compact. revert phi H2.
-    induction L as [|psi L IH]; intros phi H2.
-    - exists 0. cbn. eapply prv_weak; try apply H2. intros B [].
-    - destruct (H1 psi) as [H|[k Hk]]; try now left.
-      + destruct IH with (psi --> phi) as [n Hn].
-        * intros B HB. apply H1. now right.
-        * apply prv_DT. eapply prv_weak; try apply H2. unfold Included, In. cbn. intuition.
-        * exists n. apply prv_DT in Hn. eapply prv_weak; try apply Hn. intros B [[]| ->]; cbn; intuition.
-      + destruct IH with (psi --> phi) as [n Hn].
-        * intros B HB. apply H1. now right.
-        * apply prv_DT. eapply prv_weak; try apply H2. unfold Included, In. cbn. intuition.
-        * exists (n + k). apply prv_DT in Hn. eapply prv_weak; try apply Hn.
-          intros B [[]| ->]; try (now left); right; eapply Lext_cum1; try eassumption; lia.
-  Qed.
-
-  Lemma Lext_mono T n n' :
-    n <= n' -> T |- list_disj (snd (Lext n)) -> T |- list_disj (snd (Lext n')).
-  Proof.
-    intros H. apply list_disj_mono. now apply Lext_cum2.
-  Qed.
-  
-  Lemma ext_nder n :
-    ~ (ext |- list_disj (snd (Lext n))).
-  Proof.
-    intros [k Hk] % ext_prv. apply (Lext_nder (k + n)).
-    apply prv_DT. apply Lext_mono with n; try lia.
-    eapply prv_cut; try apply Hk. intros B [H|H].
-    - apply prv_ctx. now left.
-    - apply prv_list_conj'. apply Lext_cum1 with k; trivial. lia.
-  Qed.
-
-  Lemma ext_ex_henk :
-    ex_henk ext.
-  Proof.
-    intros phi H. destruct (form_enum_sur (∃ phi)) as [n Hn].
-    destruct (Lext n) as [L1 L2] eqn: HL.
-    destruct (SLEM (FOCDIH_prv cX (list_conj L1 --> (∃ phi) --> list_disj L2))) eqn: HS.
-    { exfalso. apply (ext_nder n). eapply prv_MP. 2: apply prv_ctx, H. eapply prv_MP. 
-      - rewrite HL. apply (prv_weak _ _ _ f). intros psi HP. left. apply HP.
-      - change (ext |- list_conj (fst (L1, L2))). rewrite <- HL. apply ext_der. }
-    exists (proj1_sig (Lext_ex n0)). right. exists (S n). cbn.
-    rewrite HL, Hn. destruct form_all as [[]|]; try discriminate.
-    destruct form_ex as [[]|].
-    - injection e. intros <-. rewrite HS. right. left. reflexivity.
-    - contradict n2. now exists phi.
-  Qed.
-
-  Lemma ext_all_henk :
-    all_henk ext.
-  Proof.
-    intros phi HP. destruct (form_enum_sur (∀ phi)) as [n Hn].
-    destruct (Lext n) as [L1 L2] eqn: HL.
-    destruct (SLEM (FOCDIH_prv cX (list_conj L1 --> (∀ phi) ∨ list_disj L2))) eqn: HS.
-    - right. exists (S n). cbn. rewrite HL, Hn. destruct form_all as [[]|].
-      + injection e as ->. rewrite HS. now left.
-      + contradict n0. now exists phi.
-    - exfalso. apply (ext_nder (S n)). cbn. rewrite HL, Hn. destruct form_all as [[]|].
-      + injection e as ->. rewrite HS. cbn. apply prv_DI2, prv_DI1, prv_ctx. apply HP.
-      + contradict n1. now exists phi.
-  Qed.
-
-  Lemma Lext_all_in phi n :
-    form_enum n = ∀ phi -> ~ (cX |- list_conj (fst (Lext n)) --> (∀ phi) ∨ list_disj (snd (Lext n)))
-    -> ∀ phi el snd (Lext (S n)).
-  Proof.
-    intros H1 H2. cbn. destruct Lext, form_all as [[]|].
-    - destruct SLEM.
-      + exfalso. rewrite H1 in e. injection e as ->. contradiction.
-      + rewrite H1 in e. injection e as ->. now left.
-    - contradict n0. exists phi. now rewrite H1.
-  Qed.
-
-  Lemma ext_ded_clos :
-    ded_clos ext.
-  Proof.
-    intros phi HP. destruct (form_enum_sur phi) as [n <-].
-    right. exists (S n). cbn. destruct Lext eqn: HL.
-    destruct form_all as [[]|]; try destruct form_ex as [[]|]; destruct SLEM; cbn in *.
-    - rewrite e. now left.
-    - exfalso. rewrite e in HP. apply (ext_nder (S n)). eapply prv_MP; try apply HP.
-      apply list_disj_In0. apply Lext_all_in; try apply e. rewrite HL. apply n0.
-    - exfalso. rewrite e in HP. apply (ext_nder n). rewrite HL.
-      eapply prv_MP; try apply HP. eapply prv_MP; try apply (ext_der n).
-      rewrite HL. eapply prv_weak; try apply f. intros phi H. now left.
-    - rewrite e. now left.
-    - exfalso. apply (ext_nder n). rewrite HL. eapply prv_MP; try apply prv_CI.
-      + eapply prv_weak; try apply f. intros phi H. now left.
-      + apply HP.
-      + change (ext |- list_conj (fst (l, l0))). rewrite <- HL. apply (ext_der n).
-    - now left.
-  Qed.
-
-  Lemma ext_B0 :
-    ~ ext B0.
-  Proof.
-    intros H. apply (ext_nder 0). apply prv_DI1, prv_ctx, H.
-  Qed.
-
-  Lemma ext_consist :
-    consist ext.
-  Proof.
-    intros H. apply ext_B0. apply ext_ded_clos.
-    apply prv_MP with ⊥; trivial. apply EFQ.
-  Qed.
-
-  Lemma ext_nel' phi :
-    ~ ext phi -> exists n, (fun psi => w psi \/ psi = phi) |- list_disj (snd (Lext n)) \/ phi el fst (Lext n).
-  Proof.
-    intros HD. destruct (form_enum_sur phi) as [n <-].
-    exists (S n). cbn. destruct Lext eqn: HL.
-    destruct form_all as [[]|]; try destruct form_ex as [[]|]; destruct SLEM; cbn in *.
-    - right. left. now rewrite e.
-    - left. rewrite e. apply prv_DI1. apply prv_ctx. now right.
-    - left. rewrite e. apply prv_DI1. apply prv_ctx. now right.
-    - right. left. now rewrite e.
-    - left. apply prv_DI1. apply prv_ctx. now right.
-    - right. now left.
-  Qed.
-
-  Lemma ext_nel phi :
-    ~ ext phi -> exists n, (fun psi => w psi \/ psi = phi) |- list_disj (snd (Lext n)).
-  Proof.
-    intros HP. destruct (ext_nel' phi HP) as [n [H|H]].
-    - exists n. apply H.
-    - exfalso. apply HP. right. now exists n.
-  Qed.
-
-  Lemma ext_prime :
-    prime ext.
-  Proof.
-    intros phi psi HD.
-    destruct (SLEM (ext phi)), (SLEM (ext psi)); try tauto.
-    apply ext_nel in n as [n H]. apply ext_nel in n0 as [n' H'].
-    exfalso. apply (ext_nder (n + n')). eapply prv_DE.
-    - apply prv_ctx. apply HD.
-    - eapply Lext_mono; try eapply prv_weak; try apply H; try lia.
-      intros theta [HT|HT]; [ left; left | right ]; tauto.
-    - eapply Lext_mono; try eapply prv_weak; try apply H'; try lia.
-      intros theta [HT|HT]; [ left; left | right ]; tauto.
-  Qed.
-
-  Instance ext_world :
-    cworlds.
-  Proof.
-    unshelve econstructor.
-    - exact ext.
-    - apply ext_consist.
-    - apply ext_prime.
-    - apply ext_ded_clos.
-    - apply ext_ex_henk.
-    - apply ext_all_henk.
-  Defined.
-
-End Lind2.
-
-(* This hypothesis follows classically from property call_henk of canonical worlds. *)
-Hypothesis w_all : forall w : cworlds, forall A, ~ w (∀ A) -> { c : nat | ~ w A[#c..] }.
-
-Lemma Lind2 : forall (cw : cworlds) A B, ~ FOCDIH_prv (fun x => cw x \/ x = A) B ->
+Lemma cwUpLind : forall (cw : cworlds) A B, ~ (FOCDIH_prv (fun x => cw x \/ x = A) B) ->
       exists (cw' : cworlds), (forall C, cw C \/ C = A -> cw' C) /\ ~ (cw' B).
 Proof.
-  intros cw A B H. exists (ext_world cw _ _ (w_all cw) H). cbn. split.
-  - intros C [HC| ->].
-    + left. apply HC.
-    + right. exists 42. apply Lext_A0.
-  - apply ext_B0 ; auto.
+  intros cw A B H.
+  eapply Up_Lindenbaum_lemma in H ; auto. destruct H ; repeat destruct p.
+  epose (Build_cworlds x _ p d e a). exists c0. split ; auto.
+  intros. destruct H ; subst ; auto. apply x0 ; auto.
+  apply cconsist. apply cprime. apply cded_clos. apply cex_henk. apply call_henk.
+  Unshelve. auto.
 Qed.
+
 
 Lemma truth_lemma : forall A (cw : cworlds),
   (ksat cw var A) <-> (cw A).
 Proof.
-pose (form_ind_subst (fun x => forall (cw : cworlds), (Canon_model ⊩( cst_ass, term) cw) var x <-> cw x)).
+pose (form_ind_subst (fun x => forall (cw : cworlds), ksat cw var x <-> cw x)).
 apply i ; clear i ; auto.
 (* ⊥ *)
 - intros cw. split ; intro.
@@ -635,63 +134,68 @@ apply i ; clear i ; auto.
   * split ; intro.
     + destruct H. rewrite IHf1 in H. rewrite IHf2 in H0. apply cded_clos.
        eapply MP. eapply MP. eapply MP. apply Ax ; eapply A8 ; reflexivity.
-       apply imp_Id_gen. eapply MP. apply Thm_irrel. 1-2: apply Id ; auto.
+       apply imp_Id_gen. eapply MP. apply Thm_irrel. all: apply Id ; auto.
     + split.
-       apply IHf1. apply cded_clos.
-       eapply MP. apply Ax ; eapply A6 ; reflexivity. apply Id ; exact H.
+       apply IHf1. apply cded_clos. eapply MP. apply Ax ; eapply A6 ; reflexivity.
+       apply Id ; exact H.
        apply IHf2. apply cded_clos. eapply MP. apply Ax ; eapply A7 ; reflexivity.
        apply Id ; exact H.
 (* f1 ∨ f2 *)
   * split ; intro.
     + destruct H.
-       rewrite IHf1 in H. apply cded_clos. eapply MP.
-       apply Ax ; eapply A3 ; reflexivity. apply Id ; auto.
-       rewrite IHf2 in H. apply cded_clos. eapply MP.
-       apply Ax ; eapply A4 ; reflexivity. apply Id ; auto.
+       rewrite IHf1 in H. apply cded_clos.
+       eapply MP. apply Ax ; eapply A3 ; reflexivity. apply Id ; auto.
+       rewrite IHf2 in H. apply cded_clos.
+       eapply MP. apply Ax ; eapply A4 ; reflexivity. apply Id ; auto.
     + apply cprime in H. rewrite IHf1 ; rewrite IHf2 ; auto.
 (* f1 --> f2 *)
   * split ; intro.
-    + destruct (classic (cw (f1 --> f2))) ; auto. exfalso.
-       assert (FOCDIH_prv (Union _ cw (Singleton _ f1)) f2 -> False).
+    + destruct (LEM (cw (f1 --> f2))) ; auto. exfalso.
+       assert ((FOCDIH_prv (Union _ cw (Singleton _ f1)) f2) -> False).
        intro. eapply FOCDIH_Deduction_Theorem in H1 ; simpl ; auto. apply H0.
        apply cded_clos ; auto.
-       pose (Lind2 cw f1 f2). destruct e.
+       pose (cwUpLind cw f1 f2). destruct e.
        intro. apply H1. eapply (FOCDIH_monot _ _ H2). intros A HA. inversion HA.
        apply Union_introl ; auto. subst. apply Union_intror ; apply In_singleton.
        destruct H2. apply H3. apply IHf2 ; auto. apply H ; auto. apply IHf1 ; auto.
-    + intros. apply IHf2. apply IHf1 in H1. apply cded_clos. eapply MP.
-       apply Id ; apply H0 ; exact H. apply Id ; auto.
+    + intros. apply IHf2. apply IHf1 in H1. apply cded_clos.
+       eapply MP. apply Id ; apply H0 ; exact H. apply Id ; auto.
 (* Quantifiers *)
 - destruct q.
   (* Universal *)
   * split ; intros.
-    + apply call_henk. intros. apply H. apply ksat_comp. apply ksat_ext with (rho:= (#c)..) ; auto.
-       intros. unfold funcomp. unfold scons. destruct x. pose (subst_term_var (#c)) ; auto. simpl. auto.
-    + simpl. intros. assert (In form cw f2[j..]). apply cded_clos. eapply MP.
-       apply Ax ; eapply A11 ; reflexivity. apply Id ; auto.
+    + apply all_henk'. apply LEM. apply call_henk. intros. apply H. apply ksat_comp. apply ksat_ext with (rho:= ($c)..) ; auto.
+       intros. unfold funcomp. unfold scons. destruct x. pose (subst_term_var ($c)) ; auto. simpl. auto.
+    + simpl. intros. assert (In form cw f2[j..]). apply cded_clos.
+       eapply MP. apply Ax ; eapply QA2 ; reflexivity. apply Id ; auto.
        apply H in H1. apply ksat_comp in H1. apply ksat_ext with (rho:= j..) in H1 ; auto.
        intros. destruct x ; auto. cbn. pose (subst_term_var j). rewrite universal_interp_eval. auto.
   (* Existential *)
   * split ; intros.
     + destruct H0. apply ksat_ext with (rho:= (x.. >> eval var)) in H0. apply ksat_comp in H0.
-       apply H in H0. apply cded_clos. eapply MP. apply Ax ; eapply A12 ; reflexivity.
-       apply Id ; exact H0.
+       apply H in H0. apply cded_clos.
+       eapply MP. apply Ax ; eapply QA3 ; reflexivity. apply Id ; exact H0.
        intros. destruct x0 ; auto. cbn. pose (subst_term_var x). rewrite universal_interp_eval. auto.
-    + simpl. apply cex_henk in H0. destruct H0. exists (#x). apply H in H0.
-       apply ksat_comp in H0. apply ksat_ext with (rho:= #x..) in H0 ; auto.
+    + simpl. apply cex_henk in H0. destruct H0. exists ($x). apply H in c.
+       apply ksat_comp in c. apply ksat_ext with (rho:= $x..) in c ; auto.
        intros. destruct x0 ; auto.
 Qed.
 
-Theorem quasi_completeness : forall A, cst_free A -> ~ FOCDIH_prv (Empty_set _) A -> ~ loc_conseq (Empty_set _) A.
+Theorem quasi_completeness : forall X A, closed_S X -> closed A -> ~ FOCDIH_prv X A -> ~ loc_conseq X A.
 Proof.
-intros A cstf notder csq. apply Lind1 in notder as [cw H] ; auto.
-apply H. apply truth_lemma. apply csq. firstorder.
+intros X A cstS cstf notder csq. apply cwTradLind in notder as [cw H] ; auto. destruct H.
+apply H. apply truth_lemma. apply csq.
+intros. apply truth_lemma ; apply H0 ; auto.
 Qed.
 
-Theorem completeness : forall A, cst_free A -> loc_conseq (Empty_set _) A -> FOCDIH_prv (Empty_set _) A.
+Theorem Completeness : forall X A, closed_S X -> closed A ->
+          loc_conseq X A -> FOCDIH_prv X A.
 Proof.
-intros A cstf csq. destruct (classic (Empty_set form |- A)); trivial.
-now apply quasi_completeness in H.
+intros X A cstS cstf csq. destruct (SLEM (X |- A)) ; [auto | exfalso].
+apply quasi_completeness in n ; auto.
 Qed.
+
+
+Print Assumptions Completeness.
 
 End completeness.
