theories/FOcdint/FOCDIH_properties.v
@@ -16,6 +16,13 @@ Section Properties.
   Context {Σ_funcs : funcs_signature}.
   Context {Σ_preds : preds_signature}.
 
+  Context {eq_dec_preds : EqDec Σ_preds}.
+  Context {eq_dec_funcs : EqDec Σ_funcs}.
+
+Notation "x 'el' L" := (List.In x L) (at level 70).
+Notation "T |- phi" := (FOCDIH_prv T phi) (at level 80).
+Notation adj T phi := (fun psi => T psi \/ psi = phi).
+
 
 Lemma Thm_irrel : forall A B Γ, FOCDIH_prv Γ (A --> (B --> A)).
 Proof.
@@ -317,7 +324,7 @@ intros L B D. induction D ; intros C Γ0 id ; subst.
   inversion H ; subst. right ; apply In_singleton. inversion H ; subst.
   destruct H0 as (B & HB0 & HB1) ; subst. exists B ; split ; auto. left ; auto.
   inversion H0 ; subst. exists C ; firstorder. right ; apply In_singleton.
-  eapply MP. apply Ax ; eapply A10 with C A. reflexivity.
+  eapply MP. apply Ax ; eapply QA1 with C A. reflexivity.
   apply Gen ; auto.
 (* EC *)
 - assert (FOCDIH_prv (fun x : form => exists B : form, x = B[↑] /\ In form Γ0 B) (C[↑] --> A --> B[↑])).
@@ -368,6 +375,16 @@ assert (Singleton form B f0). apply Hl1 ; auto. inversion H ; subst.
 inversion H0 ; subst. inversion Hl0 ; subst. apply H3 ; apply in_eq.
 Qed.
 
+
+
+
+
+
+
+
+
+Section remove_stuff.
+
 Lemma In_remove : forall (A : form) B (l : list (form)), List.In A (remove eq_dec_form B l) -> List.In A l.
 Proof.
 intros A B. induction l.
@@ -415,12 +432,15 @@ induction l.
     apply monotL_Or. apply Ax ; eapply A4 ; reflexivity.
 Qed.
 
+End remove_stuff.
 
 
-(* ------------------------------------------------------------------------------------------------------ *)
 
-(* Some proof-theoretical results about list_disj. They are helpful in the manipulation
-    of prime theories. *)
+
+
+
+
+Section list_disj_stuff.
 
 Lemma Id_list_disj : forall Γ l0 l1,
   FOCDIH_prv Γ (list_disj l0 --> list_disj (l0 ++ l1)).
@@ -589,19 +609,40 @@ destruct (in_dec eq_dec_form a l).
   auto.
 Qed.
 
+Lemma forall_list_disj : forall l Γ A,
+  FOCDIH_prv Γ (list_disj l) ->
+  (forall B, List.In B l -> FOCDIH_prv Γ (B --> A)) ->
+  FOCDIH_prv Γ A.
+Proof.
+induction l ; cbn ; intros ; auto.
+- eapply MP. apply EFQ. auto.
+- eapply MP. eapply MP. eapply MP.
+  apply Ax ; eapply A5 ; reflexivity.
+  apply H0. left ; reflexivity.
+  apply FOCDIH_Deduction_Theorem. apply IHl.
+  apply Id. right ; apply In_singleton.
+  intros. apply FOCDIH_monot with Γ. apply H0 ; auto.
+  intros C HC ; left ; auto. auto.
+Qed.
 
-(* ------------------------------------------------------------------------------------------------------ *)
+End list_disj_stuff.
 
-(* Some proof-theoretical results about list_conj. *)
+
+
+
+
+
+
+Section list_conj_stuff.
 
 Lemma list_conj_in_list : forall Γ l A,
   List.In A l ->
   FOCDIH_prv Γ ((list_conj l) --> A).
 Proof.
-induction l ; cbn ; intros ; try contradiction.
-destruct H ; subst. apply Ax ; eapply A6 ; reflexivity.
-apply IHl in H. eapply MP. eapply MP. apply Imp_trans.
-apply Ax ; eapply A7 ; reflexivity. auto.
+induction l.
+- intros. inversion H.
+- intros. cbn. inversion H. subst. apply Ax ; eapply A6 ; reflexivity. apply IHl in H0.
+  eapply MP. eapply MP. apply Imp_trans. apply Ax ; eapply A7 ; reflexivity. auto.
 Qed.
 
 Lemma finite_context_list_conj : forall Γ A,
@@ -609,8 +650,8 @@ Lemma finite_context_list_conj : forall Γ A,
   forall l, (forall A : form, (Γ A -> List.In A l) * (List.In A l -> Γ A)) ->
   FOCDIH_prv (Singleton _ (list_conj l)) A.
 Proof.
-intros. apply (FOCDIH_comp _ _ H (Singleton form (list_conj l))).
-intros. eapply MP. apply list_conj_in_list. apply H0 ; auto.
+intros. apply (FOCDIH_comp _ _ H (Singleton form (list_conj l))). intros B HB.
+eapply MP. apply list_conj_in_list. apply H0 ; exact HB.
 apply Id. apply In_singleton.
 Qed.
 
@@ -618,19 +659,22 @@ Lemma der_list_conj_finite_context : forall l (Γ : Ensemble _),
   (forall B : form, (Γ B -> List.In B l) * (List.In B l -> Γ B)) ->
   FOCDIH_prv Γ (list_conj l).
 Proof.
-induction l ; cbn ; intros.
-- apply imp_Id_gen.
-- destruct (In_dec l a).
-  + eapply MP. eapply MP. eapply MP. apply Ax ; eapply A8 ; reflexivity.
-     eapply MP. apply Thm_irrel. apply Id ; firstorder. apply imp_Id_gen.
-     apply IHl. intros. split ; intro. apply H in H0. inversion H0. subst. auto. auto.
-     apply H. apply in_cons ; auto.
-  + eapply MP. eapply MP. eapply MP. apply Ax ; eapply A8 ; reflexivity.
-     eapply MP. apply Thm_irrel. apply Id ; firstorder. apply imp_Id_gen.
-     apply FOCDIH_monot with (Γ:=(fun x : form => In form Γ x /\ x <> a)). apply IHl ; auto.
-     split ; intro. destruct H0. apply H in H0. inversion H0. subst. contradiction. auto. split ; auto.
-     apply H ; auto. intro ; subst. auto.
-     intros C HC. firstorder.
+induction l ; intros.
+- cbn. apply prv_Top.
+- cbn. destruct (In_dec l a).
+  + assert (forall B : form, (Γ B -> List.In B l) * (List.In B l -> Γ B)).
+     intros. split ; intro. apply H in H0. inversion H0. subst. auto. auto.
+     apply H. apply in_cons ; auto. pose (IHl Γ H0).
+     eapply MP. eapply MP. eapply MP. apply Ax ; eapply A8 ; reflexivity.
+     eapply MP. apply Thm_irrel. apply Id. apply H ; apply in_eq. apply imp_Id_gen. auto. 
+  + assert (J1: (forall B : form, ((fun x : form => In form Γ x /\ x <> a) B -> List.In B l) * (List.In B l -> (fun x : form => In form Γ x /\ x <> a) B))).
+     intros. split ; intro. destruct H0. apply H in H0. inversion H0. subst. exfalso. apply H1 ; auto. auto.
+     split. apply H. apply in_cons ; auto. intro. subst. auto.
+     pose (IHl (fun x => In _ Γ x /\ x <> a) J1).
+     eapply MP. eapply MP. eapply MP. apply Ax ; eapply A8 ; reflexivity.
+     eapply MP. apply Thm_irrel. apply Id. apply H ; apply in_eq. apply imp_Id_gen.
+     apply FOCDIH_monot with (Γ1:=Γ) in f0. apply f0. intros C HC.
+     inversion HC. auto.
 Qed.
 
 Lemma list_conj_finite_context : forall l (Γ : Ensemble _) A,
@@ -639,13 +683,238 @@ Lemma list_conj_finite_context : forall l (Γ : Ensemble _) A,
   FOCDIH_prv Γ A.
 Proof.
 intros.
-assert (FOCDIH_prv (Singleton form (list_conj l)) (list_conj l)). apply Id. apply In_singleton.
-assert (forall A : form, In form (Singleton form (list_conj l)) A -> FOCDIH_prv Γ A).
-intros. inversion H2 ; subst. apply der_list_conj_finite_context ; auto.
-pose (FOCDIH_comp (Singleton form (list_conj l)) A H0 Γ H2). cbn in f. auto.
+apply FOCDIH_comp with (Γ:=(Singleton form (list_conj l))) ; auto.
+intros. inversion H1 ; subst. apply der_list_conj_finite_context.
+intro B ; split ; intro HB ; apply H ; auto.
 Qed.
 
+End list_conj_stuff.
+
+
+
+
+Section Prv.
+
+  Lemma prv_ctx (T : form -> Prop) phi :
+    T phi -> T |- phi.
+  Proof.
+    intros H. apply Id. auto.
+  Qed.
+
+  Lemma prv_weak T T' A :
+    T |- A -> Included _ T T' -> T' |- A.
+  Proof.
+    intros H1 H2. eapply FOCDIH_monot in H1; eassumption.
+  Qed.
+
+  Lemma prv_MP {T : form -> Prop} {phi} psi :
+    T |- psi --> phi -> T |- psi -> T |- phi.
+  Proof.
+    intros H1 H2. eapply MP ; auto.
+    - exact H1.
+    - auto.
+  Qed.
+
+  Lemma prv_DT T A B :
+    adj T A |- B <-> T |- A --> B.
+  Proof.
+    split; intros HT.
+    - apply FOCDIH_Deduction_Theorem.
+      eapply prv_weak; try apply HT. intros C [HC| ->]; [ left | right ]; trivial. constructor.
+    - apply prv_MP with A; try (apply prv_ctx; now right). eapply prv_weak; try apply HT. firstorder.
+  Qed.
+
+  Lemma prv_compact T A :
+    T |- A -> exists L, (forall B, B el L -> T B) /\ (fun B => B el L) |- A.
+  Proof.
+    intros (T' & H1 & H2 & L & HL) % FOCDIH_finite. exists L. split; intuition.
+    eapply prv_weak; try apply H2. intuition.
+  Qed.
+
+  Lemma prv_cut T T' A :
+    T |- A -> (forall B, T B -> T' |- B) -> T' |- A.
+  Proof.
+    intros [L [H1 H2]] % prv_compact H. induction L in A, H1, H2 |- *.
+    - eapply prv_weak; try apply H2. intros B [].
+    - eapply prv_MP; try apply (IHL (a --> A)).
+      + intros B HB. apply H1. now right.
+      + apply prv_DT. eapply prv_weak; try apply H2. intros B [->| HB]; cbn; intuition.
+      + apply H, H1. now left.
+  Qed.
+
+  Lemma prv_EI {T : form -> Prop} {phi} t :
+    T |- phi[t..] -> T |- ∃ phi.
+  Proof.
+    intros H. eapply prv_MP; try apply H. constructor 2.
+    econstructor 12 ; reflexivity.
+  Qed.
+
+   Lemma prv_EE T A B :
+    (fun C => exists C', C = C'[↑] /\ T C') |- A --> B[↑] -> T |- (∃ A) --> B.
+  Proof.
+    intros H. eapply EC; try apply ECRule_I ; auto.
+  Qed.
+
+  Lemma prv_AI T A :
+    (fun C => exists C', C = C'[↑] /\ T C') |- A -> T |- ∀ A.
+  Proof.
+    intros H. eapply Gen; try apply GenRule_I ; auto.
+  Qed.
+
+  Lemma prv_AE {T : form -> Prop} {phi} t :
+    T |- ∀ phi -> T |- phi[t..].
+  Proof.
+    intros H. eapply prv_MP; try apply H. constructor 2.
+    econstructor 11 ; reflexivity.
+  Qed.
+
+  Lemma prv_DI1 T A B :
+    T |- A -> T |- A ∨ B.
+  Proof.
+    intros H. eapply prv_MP; try apply H. constructor 2.
+    econstructor 3 ; reflexivity.
+  Qed.
+
+  Lemma prv_DI2 T A B :
+    T |- B -> T |- A ∨ B.
+  Proof.
+    intros H. eapply prv_MP; try apply H. constructor 2.
+    econstructor 4 ; reflexivity.
+  Qed.
+
+  Lemma prv_DE T phi psi theta :
+    T |- phi ∨ psi -> adj T phi |- theta -> adj T psi |- theta -> T |- theta.
+  Proof.
+    intros H1 H2 H3. eapply prv_MP. eapply prv_MP. eapply prv_MP.
+    - constructor 2. econstructor 5 ; reflexivity.
+    - apply prv_DT. apply H2.
+    - apply prv_DT. apply H3.
+    - apply H1.
+  Qed.
+
+  Lemma prv_CI T A B :
+    T |- A -> T |- B -> T |- A ∧ B.
+  Proof.
+    intros H1 H2. eapply prv_MP. eapply prv_MP. eapply prv_MP.
+    - constructor 2. econstructor 8 ; reflexivity.
+    - apply prv_DT. apply prv_ctx. now right.
+    - eapply MP. apply Thm_irrel. auto.
+    - apply H1.
+  Qed.
+
+  Lemma prv_CE1 T A B :
+    T |- A ∧ B -> T |- A.
+  Proof.
+    intros H. eapply prv_MP; try apply H. constructor 2.
+    econstructor 6 ; reflexivity.
+  Qed.
+
+  Lemma prv_CE2 T A B :
+    T |- A ∧ B -> T |- B.
+  Proof.
+    intros H. eapply prv_MP; try apply H. constructor 2.
+    econstructor 7 ; reflexivity.
+  Qed.
+
+  Lemma prv_exp T A :
+    T |- ⊥ -> T |- A.
+  Proof.
+    intros H. eapply prv_MP; try apply H. constructor 2.
+    econstructor 9 ; reflexivity.
+  Qed.
+
+  Lemma prv_cas_car T A B C :
+    T |- A --> B --> C <-> T |- B ∧ A --> C.
+  Proof.
+    split; intros H.
+    - apply prv_DT. eapply prv_MP. eapply prv_MP.
+      + eapply prv_weak; try apply H. firstorder.
+      + eapply prv_CE2, prv_ctx. now right.
+      + eapply prv_CE1, prv_ctx. now right.
+    - apply prv_DT. apply -> prv_DT. eapply prv_MP.
+      + eapply prv_weak; try apply H. firstorder.
+      + apply prv_CI; apply prv_ctx; firstorder.
+  Qed.
+
+  Lemma prv_list_conj T L :
+    (forall A, A el L -> T |- A) -> T |- list_conj L.
+  Proof.
+    intros H. induction L.
+    - apply prv_Top.
+    - cbn. apply prv_CI.
+      + apply H. now left.
+      + apply IHL. firstorder.
+  Qed.
+
+  Lemma prv_list_conj' T L A :
+    A el L -> adj T (list_conj L) |- A.
+  Proof.
+    induction L; cbn; try tauto. intros [-> | H].
+    - eapply prv_CE1. apply prv_ctx. now right.
+    - apply prv_DT in IHL; trivial. eapply prv_MP.
+      + eapply prv_weak; try apply IHL. firstorder.
+      + eapply prv_CE2. apply prv_ctx. now right.
+  Qed.
+
+  Lemma prv_list_disj T L A :
+    A el L -> T |- A -> T |- list_disj L.
+  Proof.
+    induction L; cbn; try now intros []. intros [-> |H] HA.
+    - apply prv_DI1. apply HA.
+    - apply prv_DI2. now apply IHL.
+  Qed.
+
+  Lemma list_disj_mono T L L' :
+    incl L L' -> T |- list_disj L -> T |- list_disj L'.
+  Proof.
+    induction L in T |- *; cbn; intros H1 H2.
+    - apply prv_exp. apply H2.
+    - eapply prv_DE; try apply H2.
+      + apply prv_list_disj with a; try firstorder. apply prv_ctx. now right.
+      + apply IHL; try firstorder. apply prv_ctx. now right.
+  Qed.
+
+  Lemma Lext_ex_der {T L1 L2 psi} c :
+    T |- list_conj (∃ psi :: psi[$c..] :: L1) --> list_disj L2
+        -> T |- list_conj L1 --> psi[$c..] --> list_disj L2.
+  Proof.
+    intros H. apply prv_DT. apply -> prv_DT. apply prv_DT in H.
+    eapply prv_cut; try apply H. intros B [HB | ->].
+    - apply prv_ctx. left. now left.
+    - cbn. apply prv_CI; try apply prv_CI.
+      + eapply prv_EI. apply prv_ctx. now right.
+      + apply prv_ctx. now right.
+      + apply prv_ctx. left. now right.
+  Qed.
+
+  Lemma Lext_all_der {T L1 L2 psi} c :
+    T |- list_conj L1 --> list_disj (∀ psi :: psi[$c..] :: L2)
+        -> T |- list_conj L1 --> psi[$c..] ∨ list_disj L2.
+  Proof.
+    intros H. apply prv_DT. apply prv_DT in H.
+    cbn in H. eapply prv_DE; try apply H.
+    - apply prv_DI1. apply prv_AE. apply prv_ctx. now right.
+    - apply prv_ctx. now right.
+  Qed.
+
+End Prv.
+
+
 (* Having Cut is quite convenient. *)
+
+Lemma Or_imp_assoc : forall A B C D Γ,
+  FOCDIH_prv Γ (A --> ((B ∨ C) ∨ D)) ->
+  FOCDIH_prv Γ (A --> (B ∨ (C ∨ D))).
+Proof.
+intros. eapply MP. eapply MP. apply Imp_trans. exact H.
+eapply MP. eapply MP. apply Ax ; eapply A5 ; reflexivity.
+eapply MP. eapply MP. apply Ax ; eapply A5 ; reflexivity.
+apply Ax ; eapply A3 ; reflexivity. eapply MP. eapply MP.
+apply Imp_trans. apply Ax ; eapply A3 ; reflexivity.
+apply Ax ; eapply A4 ; reflexivity. eapply MP.
+eapply MP. apply Imp_trans. apply Ax ; eapply A4 ; reflexivity.
+apply Ax ; eapply A4 ; reflexivity.
+Qed.
 
 Lemma Cut : forall (Γ Δ: @Ensemble (form)) A,
         pair_der (Union _ Γ (Singleton _ A)) Δ  ->
@@ -673,20 +942,8 @@ eapply MP. 2: exact f.
 eapply MP. apply Imp_trans. auto.
 Qed.
 
-Lemma Or_imp_assoc : forall A B C D Γ,
-  FOCDIH_prv Γ (A --> ((B ∨ C) ∨ D)) ->
-  FOCDIH_prv Γ (A --> (B ∨ (C ∨ D))).
-Proof.
-intros. eapply MP. eapply MP. apply Imp_trans. exact H.
-eapply MP. eapply MP. apply Ax ; eapply A5 ; reflexivity.
-eapply MP. eapply MP. apply Ax ; eapply A5 ; reflexivity.
-apply Ax ; eapply A3 ; reflexivity. eapply MP. eapply MP.
-apply Imp_trans. apply Ax ; eapply A3 ; reflexivity.
-apply Ax ; eapply A4 ; reflexivity. eapply MP.
-eapply MP. apply Imp_trans. apply Ax ; eapply A4 ; reflexivity.
-apply Ax ; eapply A4 ; reflexivity.
-Qed.
 
 End Properties.
+
 
 
