theories/FOcdint/FO_CDInt_soundness.v
@@ -14,14 +14,20 @@ Local Unset Strict Implicit.
 
 Section Soundness_LEM.
 
-Axiom LEM : forall P, P \/ ~ P.
-
   Context {Σ_funcs : funcs_signature}.
   Context {Σ_preds : preds_signature}.
 
+Axiom LEM : forall P, P \/ ~ P.
+
+Lemma ksat_dec : forall A D (M : kmodel D) u rho,
+    (@ksat _ _ D M u rho A) \/ ((ksat u rho A) -> False).
+Proof.
+intros. apply LEM.
+Qed.
+
 Lemma Ax_valid : forall A, Axioms A -> kvalid A.
 Proof.
-intros A AX. inversion AX ; subst ; intros w alpha ass u rho ; cbn ; intros ; auto.
+intros A AX. inversion AX ; subst ; intros w M u rho ; cbn ; intros ; auto.
 - apply ksat_mon with v ; auto.
 - apply H0 with v1 ; auto. apply reach_tran with v0 ; auto. apply reach_refl.
 - destruct H4. apply H0 ; auto. apply (reach_tran H1 H3). apply H2 ; auto.
@@ -29,35 +35,36 @@ intros A AX. inversion AX ; subst ; intros w alpha ass u rho ; cbn ; intros ; au
 - destruct H0 ; auto.
 - split. apply H0 ; auto. apply (reach_tran H1 H3). apply H2 ; auto.
 - inversion H0.
+(* Quantifiers *)
 - apply H0 ; auto. apply ksat_comp ; auto.
-- apply ksat_comp. unfold funcomp. eapply (ksat_ext alpha v). 2: eapply (H0 (eval rho _)).
+- apply ksat_comp. unfold funcomp. eapply (ksat_ext v). 2: eapply (H0 (eval rho _)).
   intros. unfold scons. destruct x ; auto.
-- apply ksat_comp in H0. eexists (eval rho t). eapply (ksat_ext _ v). 2: eapply H0.
+- apply ksat_comp in H0. eexists (eval rho t). eapply (ksat_ext v). 2: eapply H0.
   unfold funcomp. intros. unfold scons. destruct x ; auto.
-- destruct (LEM ((ass ⊩( alpha, w) v) rho B)) ; auto. (* Use of LEM *)
+- destruct (LEM ((v ⊩( M, w) rho) B)) ; auto. (* Use of LEM *)
   left. intros. destruct (H0 j) ; auto. exfalso. apply H1. apply ksat_comp in H2.
-  eapply (ksat_ext _ v). 2: exact H2. intros. unfold funcomp. unfold scons.
+  eapply (ksat_ext v). 2: exact H2. intros. unfold funcomp. unfold scons.
   cbn ; auto.
 Qed.
 
 Lemma Soundness : forall Γ A, FOCDIH_prv Γ A -> loc_conseq Γ A.
 Proof.
-intros Γ A Hprv. induction Hprv; subst; cbn; intros D M u ass rho HX.
+intros Γ A Hprv. induction Hprv; subst; cbn; intros D M u rho HX.
 (* Id *)
 - apply HX ; auto.
 (* Ax *)
 - apply Ax_valid ; auto.
 (* MP *)
-- unfold kvalid_ctx in IHHprv1,IHHprv2. pose (IHHprv1 _ _ _ _ _ HX). pose (IHHprv2 _ _ _ _ _ HX).
+- unfold kvalid_ctx in IHHprv1,IHHprv2. pose (IHHprv1 _ _ _ _ HX). pose (IHHprv2 _ _ _ _ HX).
   simpl in k. apply k ; auto. apply reach_refl.
 (* Gen *)
 - intro d. unfold kvalid_ctx in IHHprv. apply IHHprv. intros. inversion H. destruct H0 ; subst.
   apply HX in H1. apply ksat_comp. simpl. unfold funcomp. simpl. auto.
 (* EC *)
 - intros ass0 Ha0 Ha1. unfold loc_conseq in IHHprv. destruct Ha1.
-  assert (J2: (forall psi : form, (fun x : form => exists B : form, x = B[↑] /\ In form Γ B) psi -> (u ⊩( M, D) ass) (x .: rho) psi)). intros.
+  assert (J2: (forall psi : form, (fun x : form => exists B : form, x = B[↑] /\ In form Γ B) psi -> (u ⊩( M, D) (x .: rho)) psi)). intros.
   destruct H0. destruct H0. subst. apply HX in H1. apply ksat_comp.
-  simpl. unfold funcomp. simpl. auto. pose (IHHprv _ _ u _ (x .: rho) J2).
+  simpl. unfold funcomp. simpl. auto. pose (IHHprv _ _ u (x .: rho) J2).
   simpl in k. apply k in H ; auto. apply ksat_comp in H. unfold funcomp in H. simpl in H. auto.
 Qed.
 
